Refinement attempt 1

denotational/Examples.v
@@ -9,16 +9,23 @@ From Coq Require Import
 
 From ExtLib Require Import
      RelDec
-     Functor
+     Maps
+     FMapAList
+     Reducible
      Traversable
      Monads
      Option.
 
 From CTree Require CTrees.
 
+From CTree Require Import
+     Equ
+     Utils.
+
 From DSL Require Import
      System
      Network
+     Refinement
      Vectors.
 
 Import ITreeNotations.
@@ -61,13 +68,44 @@ Module Examples.
     a <- load "a";;
     store "b" (S (default a 0)).
 
-  Definition S1 := [example].
-  Definition S2 := [example_alice; example_bob].
+  (** Here we are evaluating two distributed systems to CTrees C1, C2.
+      We will show they are equivalent by some sort of Applicative Bisimulation
+      using the leaf equivalence below. *)
 
-  Definition C1 := run_network (run_storage S1) List.nil.
-  Definition C2 := run_network (run_storage S2) List.nil.
+  Definition init_heap :=(List.cons ("a", 0) List.nil).
+  Definition C1 := run_network (run_storage [example]) init_heap.
+  Definition C2 := run_network (run_storage [example_alice; example_bob]) init_heap.
 
-  Check C1.
-  Check C2.
+  (** Extensional equality of Maps *)
+  Global Instance RelDec_Maps_ext {K V M} `{m: Maps.Map K V M} `{Foldable M (K * V)}
+           `{RelDec K (@eq K)} `{RelDec V (@eq V)} : RelDec (@eq M) := {
+      rel_dec a b := let left :=
+                       fold (fun '(k, v) acc =>
+                               andb acc (rel_dec (Maps.lookup k b) (Some v))
+                            ) true a in
+                     let right :=
+                       fold (fun '(k, v) acc =>
+                               andb acc (rel_dec (Maps.lookup k a) (Some v))
+                            ) true b in
+                     andb left right
+    }.
+
+  (** Heterogenous Equivalence that only looks at state of agent 1 in either system.
+      Applied on leaves of CTree. *)
+  Equations vec_head_heap_equiv{n m A B}(a: vec (S n) (heap * (A * queue (S n))))
+            (b: vec (S m) (heap * (B * queue (S m)))): Prop :=
+    vec_head_heap_equiv ((ha, _) :: _ ) ((hb, _) :: _) := rel_dec ha hb = true.
+  Transparent vec_head_heap_equiv.
+
+  Notation "a '~1h~' b" := (vec_head_heap_equiv a b) (at level 90, left associativity).
+
+  Lemma refinement_c1_c2: refinement vec_head_heap_equiv C2 C1.
+  Proof.
+    unfold C2, C1, example, example_alice, example_bob, run_network, run_storage.
+    cbn.
+    (** LOOPS HERE *)
+    rewrite rewrite_schedule.
+
+
 End Examples.
     
