denotational/Refinement.v
@@ -1,0 +1,43 @@
+
+From CTree Require Import
+     CTrees
+     Utils.
+
+From ITree Require Import
+     Indexed.Sum.
+
+From Coq Require Import
+     Fin (* fin definition here *)
+     Program.Equality
+     Lia.
+
+From Equations Require Import
+     Equations.
+
+Import CTreeNotations.
+Local Open Scope ctree_scope.
+
+Set Implicit Arguments.
+Set Contextual Implicit.
+
+(** A relation transformer that lifts an R: A -> B -> Prop 
+    to a ctree void1 A -> ctree void1 B -> Prop. Not sure if it
+    is correct but the intuition is 
+    
+    refinement R a b := 
+        (1) a has the same or more choices than b on the branches.
+        (2) R a b holds on the leaves
+*)
+Inductive refinement{A B} (R: A -> B -> Prop):
+  ctree void1 A -> ctree void1 B -> Prop :=
+| RetRet: forall a b, R a b -> refinement R (Ret a) (Ret b)
+| RetChoice: forall b n (k: fin n -> ctree void1 B) a,
+  (forall f, refinement R (Ret a) (k f)) ->
+  refinement R (Ret a) (Choice b n k)
+| ChoiceRet: forall b n (k: fin n -> ctree void1 A) a,
+  (exists f, refinement R (k f) (Ret a)) ->
+  refinement R (Choice b n k) (Ret a)
+| ChoiceChoice: forall b n1 n2 (k1: fin n1 -> ctree void1 A)
+                       (k2: fin n2 -> ctree void1 B),
+    (forall f2, exists f1, refinement R (k1 f1) (k2 f2)) ->
+    refinement R (Choice b n1 k1) (Choice b n2 k2).
